Changes

imperative-stuff.dfy
@@ -1,1 +1,39 @@
+function method sum_squares(n: nat): nat
+{
+    if n == 0 then 0
+    else n * n + sum_squares( n - 1 )
+}
 
+ method sum_squares_verified(n: nat) returns (f: nat)
+    ensures f == sum_squares(n)
+ {
+     if ( n == 0 )
+     {
+         return 0;
+     }
+
+     assert n > 0;
+
+     var i := n;
+     var a := 0;
+
+     while( i > 0 )
+        invariant 0 <= i <= n;
+        invariant a + sum_squares(i) == sum_squares(n);
+     {
+        a := a + ( i * i );
+        i := i - 1;
+     }
+
+     assert !( i > 0 );
+     assert a == sum_squares(n);
+
+     return a;
+ }
+
+method Main()
+{
+    print "sum_squares(5) is ", sum_squares(5), "\n";
+    var att := sum_squares_verified(5);
+    print "sum_squares_verified(5) is ", att, "\n";
+}
